start integrating spec

Tutorial/SPI.v
@@ -1,5 +1,31 @@
-Require Import Kami.All.
+Require Import Coq.Lists.List. Import ListNotations.
+Module spec.
+  
+  Axiom one : forall {T}, (T -> Prop) -> list T -> Prop.
+  Axiom plus : forall {T}, (list T -> Prop) -> list T -> Prop.
+  Axiom app : forall {T}, (list T -> Prop) -> (list T -> Prop) -> list T -> Prop.
+  Local Notation "x ^+" := (plus x) (at level 50).
+  Local Infix "+++" := app (at level 60).
+  
+  Definition flat_map {A B} (P:A->list B->Prop) xs :=
+    List.fold_right app (eq nil) (List.map P xs).
+  
+  Definition at_next_edge {T} clk data : list T -> Prop :=
+    (fun x => not (clk x))^+ +++ (fun x => clk x /\ data x).
+  
+  Definition clk : list (bool * bool * bool) -> Prop :=
+    one (fun '(clk, _, _) => clk = true).
+  Definition mosi : bool -> list (bool * bool * bool) -> Prop :=
+    fun b => one (fun '(_, mosi, _) => mosi = b).
+  Definition miso : bool -> list (bool * bool * bool) -> Prop :=
+    fun b => one (fun '(_, _, miso) => miso = b).
+  
+  (* TODO: allow and ignore nop-s in external io *)
+  Definition mosis := @flat_map bool (bool*bool*bool) (fun x => at_next_edge clk (mosi x)).
+  Definition misos := @flat_map bool (bool*bool*bool) (fun x => at_next_edge clk (miso x)).
+End spec.
 
+Require Import Kami.All.
 Definition x : nat. exact O. Qed.
 
 Section Named.
@@ -14,29 +40,29 @@ Section Named.
     with Register @^"tx_fifo_len" : Bit 4 <- Default
     with Register @^"rx_fifo"     : Bit 8 <- Default
     with Register @^"rx_fifo_len" : Bit 4 <- Default
-    with Register @^"sck"         : Bool <- Default
+    with Register @^"sck"         : Bool  <- Default
     
     with Rule @^"cycle" := (
       Write @^"hack_for_sequential_semantics" : Bit 0 <- $$(WO);
-      Call miso : Bit 1 <- "GetMISO"();
 
       Read sck <- @^"sck";
       Read tx_fifo : Bit 8 <- @^"tx_fifo";
       Read tx_fifo_len : Bit 4 <- @^"tx_fifo_len";
       Read rx_fifo : Bit 8 <- @^"rx_fifo";
       Read rx_fifo_len : Bit 4 <- @^"rx_fifo_len";
+
+      Call miso : Bit 1 <- "GetMISO"();
+      Call "PutSCK"(#sck : Bool);
+      Call "PutMOSI"((UniBit (TruncMsb 7 1) #tx_fifo) : Bit 1);
+
       If (#tx_fifo_len == $$@natToWord 4 0) then (
         If (#sck) then (
           Write @^"tx_fifo" : Bit 8 <- UniBit (TruncLsb 8 1) (BinBit (Concat 8 1) #tx_fifo $$(@ConstBit 1 $x));
           Write @^"tx_fifo_len" <- #tx_fifo_len - $1;
-          Call "PutSCK"(#sck : Bool);
-          Call "PutMOSI"((UniBit (TruncMsb 7 1) #tx_fifo) : Bit 1);
           Retv
         ) else (
           Write @^"rx_fifo" : Bit 8 <- UniBit (TruncLsb 8 1) (BinBit (Concat 8 1) #rx_fifo #miso);
           Write @^"rx_fifo_len" : Bit 4 <- #rx_fifo_len + $1;
-          Call "PutSCK"(#sck : Bool);
-          Call "PutMOSI"((UniBit (TruncMsb 7 1) #tx_fifo) : Bit 1);
           Retv
         );
         Retv
@@ -60,7 +86,7 @@ Section Named.
     )
     
     with Method "read" () : Bool := ( (* TODO return pair *)
-      Write @^"hack_for_sequential_semantich" : Bit 0 <- $$(WO);
+      Write @^"hack_for_sequential_semantics" : Bit 0 <- $$(WO);
       Read rx_fifo <- @^"rx_fifo";
       Read rx_fifo_len <- @^"rx_fifo_len";
       If (#rx_fifo_len == $$@natToWord 4 8) then (
@@ -74,13 +100,50 @@ Section Named.
     )
   }.
 
-  (* Eval cbv -[type fullType fst snd] in FullLabel. *)
-  (* = (list RegT * (RuleOrMeth * list (string * {k : Kind * Kind & type (fst k) * type (snd k)})))%type *)
+  Definition iocycle miso sck mosi := eq (Rle (name ++ "_cycle"),
+      [("GetMISO", existT SignT (Void, Bit 1) (wzero 0, miso));
+      ("PutSCK",   existT SignT (Bool, Void)  (sck, wzero 0));
+      ("PutMOSI",  existT SignT (Bit 1, Void) (mosi, wzero 0))]).
+  Definition cmd_write arg err := eq
+    (Meth ("write", existT SignT (Bit 8, Bool) (arg, err)), @nil MethT).
+  Definition cmd_read (ret : word 8) err := eq (* TODO: use "ret" *)
+    (Meth ("read", existT SignT (Void, Bool) (wzero 0, err)), @nil MethT).
+  Definition nop x := (exists arg, cmd_write arg true x) \/ (exists ret, cmd_read ret true x).
 
-  Goal forall (P:_->Prop) r l, Trace SPI r l -> P (map (map snd) l).
+  Definition parsable := Forall (fun l => exists (r:RegsT) x, l = [(r, x)] /\
+    ((exists miso sck mosi, iocycle miso sck mosi x) \/
+     (exists arg err, cmd_write arg err x) \/
+     (exists ret err, cmd_read ret err x))).
+
+  Goal forall (I:_->Prop) r l, I r -> Trace SPI r l -> parsable l.
   Proof.
-    intros.
-    induction H; subst; [admit|].
+    intros I r l HI HTrace.
+    induction HTrace.
+    { subst ls'. cbn. admit. }
+
+    unshelve (idtac;
+    let pf := open_constr:(InvertStep (@Build_BaseModuleWf SPI _) _ _ _ HStep) in
+    destruct pf);
+    [abstract discharge_wf|..];
+    repeat match goal with
+      | _ => progress intros
+      | _ => progress clean_hyp_step
+      | _ => progress cbn [SPI getMethods baseModule makeModule makeModule' type evalExpr isEq evalConstT Kind_rect app map fst snd projT1 projT2] in *
+    end.
+    15: {
+      erewrite (word0 arg).
+      constructor.
+      2: eapply IHHTrace; admit.
+      eexists ?[r], (?[n], ?[vs]).
+      split; repeat f_equal.
+      right; right.
+      eexists _, _.
+      exact eq_refl. }
+
+
+  Abort.
+
+    (*
     inversion HStep; subst.
     inversion HSubsteps; subst.
     3: {
@@ -111,29 +174,17 @@ Section Named.
       2: { symmetry; eapply UIP_refl. }
       cbn in H2.
       clear H0.
-      rewrite @UIP_refl in H2.
-      unfold eq_rect in *.
-      
-      inv H0.
-      match goal with
-      | H:existT ?a ?b1 ?c1 = existT ?a ?b2 ?c2
-      |- _ => idtac H; apply inversionExistT in H; destruct H as [? ?]; subst
-      end.
+      repeat clean_hyp_step.
 
-      clean_hyp_step.
-      clean_hyp_step.
-      clean_hyp_step.
-      clean_hyp_step.
-      clean_hyp_step.
-      clean_hyp_step.
-      
-      admit. (* stuck on eq_refl match *)
-      admit. (* stuck on eq_refl match *)
-    }
-    2: {
+      Notation "( x , y , .. , z )" := (existT _ .. (existT _ x y) .. z) : core_scope.
+
+      all:
+      try subst method;
+      cbn [type] in *;
       repeat clean_hyp_step;
-      cbn [evalExpr isEq evalConstT Kind_rect map fst snd] in *.
-      admit.
+      cbn [evalExpr isEq evalConstT Kind_rect app map fst snd] in *.
 
+      2: {
+        *)
 
 End Named.
